Use more fine-grained normalisation assumptions in erasure

erasure/theories/ETransform.v
@@ -4,7 +4,7 @@ From Equations Require Import Equations.
 From MetaCoq.Template Require Import Transform bytestring config utils BasicAst uGraph.
 From MetaCoq.Template Require Pretty Environment Typing WcbvEval EtaExpand.
 Set Warnings "-notation-overridden".
-From MetaCoq.PCUIC Require PCUICAst PCUICAstUtils PCUICProgram PCUICTransform.
+From MetaCoq.PCUIC Require PCUICAst PCUICAstUtils PCUICProgram PCUICTransform PCUICWeakeningEnvSN.
 Set Warnings "+notation-overridden".
 From MetaCoq.SafeChecker Require Import PCUICErrors PCUICWfEnv PCUICWfEnvImpl.
 From MetaCoq.Erasure Require EAstUtils ErasureFunction ErasureCorrectness Extract
@@ -20,39 +20,161 @@ Definition build_wf_env_from_env {cf : checker_flags} (Σ : global_env_map) (wf�
      wf_env_map_repr := Σ.(trans_env_repr);
  |}.
 
-Program Definition erase_pcuic_program {guard : abstract_guard_impl} {normalisation : PCUICSN.Normalisation} (p : pcuic_program)
+
+Notation NormalisationIn_erase_pcuic_program_1 p
+  := (@PCUICTyping.wf_ext config.extraction_checker_flags p.1 -> PCUICSN.NormalisationIn (cf:=config.extraction_checker_flags) (no:=PCUICSN.extraction_normalizing) p.1)
+       (only parsing).
+
+Notation NormalisationIn_erase_pcuic_program_2 p
+  := (@PCUICTyping.wf_ext config.extraction_checker_flags p.1 -> PCUICWeakeningEnvSN.NormalisationInAdjustUniversesIn (cf:=config.extraction_checker_flags) (no:=PCUICSN.extraction_normalizing) p.1)
+       (only parsing).
+
+(* TODO: Where should this go? *)
+#[local]
+Lemma referenced_impl_env_iter_pop_eq'
+  (cf := config.extraction_checker_flags)
+  (no := PCUICSN.extraction_normalizing)
+  {guard : abstract_guard_impl}
+  (wfe : wf_env)
+  (n : nat)
+  (X' := ErasureFunction.iter abstract_pop_decls (S n) wfe)
+  (wfe' := ErasureFunction.iter referenced_pop (S n) (referenced_impl_env wfe))
+  : referenced_impl_env X' = wfe'.
+Proof.
+  subst X' wfe'.
+  revert wfe; cbn; induction n as [|n IHn]; cbn; intros;
+    [ | rewrite IHn ].
+  all: destruct wfe as [[[? [|[]]]]]; cbv [optim_pop]; cbn; reflexivity.
+Qed.
+
+#[local]
+Lemma referenced_impl_env_iter_pop_eq
+  (cf := config.extraction_checker_flags)
+  (no := PCUICSN.extraction_normalizing)
+  {guard : abstract_guard_impl}
+  (wfe : wf_env)
+  (n : nat)
+  (X' := ErasureFunction.iter abstract_pop_decls (S n) wfe)
+  : referenced_impl_env X'
+    = {| PCUICAst.PCUICEnvironment.universes := PCUICAst.PCUICEnvironment.universes (referenced_impl_env wfe)
+      ; PCUICAst.PCUICEnvironment.declarations := skipn (S n) (PCUICAst.PCUICEnvironment.declarations (referenced_impl_env wfe))
+      ; PCUICAst.PCUICEnvironment.retroknowledge := PCUICAst.PCUICEnvironment.retroknowledge (referenced_impl_env wfe) |}.
+Proof.
+  subst X'.
+  revert wfe; cbn; induction n as [|n IHn]; cbn; intros;
+    [ | rewrite IHn ].
+  all: destruct wfe as [[[? [|[]]]]]; cbv [optim_pop]; cbn; reflexivity.
+Qed.
+
+#[local] Lemma erase_pcuic_program_normalisation_helper
+  (cf := config.extraction_checker_flags) (no := PCUICSN.extraction_normalizing)
+  {guard : abstract_guard_impl} (p : pcuic_program)
+  {normalisation_in : NormalisationIn_erase_pcuic_program_1 p}
+  {normalisation_in_adjust_universes : NormalisationIn_erase_pcuic_program_2 p}
+  (wfΣ : ∥ PCUICTyping.wf_ext (H := config.extraction_checker_flags) p.1 ∥)
+  : (let wfe := build_wf_env_from_env p.1.1 (map_squash (PCUICTyping.wf_ext_wf _) (wfΣ : ∥ PCUICTyping.wf_ext (H := config.extraction_checker_flags) p.1 ∥)) in
+     forall n : nat,
+       n < #|PCUICAst.PCUICEnvironment.declarations p.1|
+      -> forall kn cb pf,
+        hd_error (skipn n (PCUICAst.PCUICEnvironment.declarations p.1)) =
+          Some (kn, PCUICAst.PCUICEnvironment.ConstantDecl cb) ->
+        forall Σ : PCUICAst.PCUICEnvironment.global_env_ext,
+          PCUICTyping.wf_ext Σ ->
+          Σ
+            ∼_ext @abstract_make_wf_env_ext extraction_checker_flags
+            (@optimized_abstract_env_impl extraction_checker_flags _) wfe
+            (PCUICAst.PCUICEnvironment.cst_universes cb) pf -> PCUICSN.NormalisationIn Σ)
+    /\
+      (let wfe := build_wf_env_from_env p.1.1 (map_squash (PCUICTyping.wf_ext_wf _) (wfΣ : ∥ PCUICTyping.wf_ext (H := config.extraction_checker_flags) p.1 ∥)) in
+       forall n : nat,
+         n < #|PCUICAst.PCUICEnvironment.declarations p.1|
+        -> let X' :=
+             ErasureFunction.iter abstract_pop_decls (S n) wfe in
+           forall kn cb pf,
+             hd_error (skipn n (PCUICAst.PCUICEnvironment.declarations p.1)) =
+               Some (kn, PCUICAst.PCUICEnvironment.ConstantDecl cb) ->
+             let Xext :=
+               @abstract_make_wf_env_ext extraction_checker_flags
+                 (@optimized_abstract_env_impl extraction_checker_flags _) X'
+                 (PCUICAst.PCUICEnvironment.cst_universes cb) pf in
+             forall Σ : PCUICAst.PCUICEnvironment.global_env_ext,
+               PCUICTyping.wf_ext Σ -> Σ ∼_ext Xext -> PCUICSN.NormalisationIn Σ).
+Proof.
+  match goal with |- ?A /\ ?B => cut (A /\ (A -> B)); [ tauto | ] end.
+  cbv beta zeta; split.
+  all: cbn; intros; subst;
+    repeat match goal with
+      | [ H : forall x, x = _ -> _ |- _ ] => specialize (H _ eq_refl)
+      | [ H : squash _ |- _ ] => destruct H
+      | [ H : ?A -> ?B, H' : ?A |- _ ] => specialize (H H')
+      end.
+  { destruct p as [Σ ?]; cbn in *.
+    match goal with H : PCUICSN.NormalisationIn _ |- _ => revert H end.
+    eapply normalisation_in_adjust_universes; try assumption.
+    cbv [PCUICSN.NormalisationIn]; cbn.
+    let H := match goal with H : PCUICTyping.wf_ext _ |- _ => H end in
+    rewrite /PCUICAst.PCUICEnvironment.lookup_env -PCUICAst.PCUICEnvironment.lookup_global_Some_iff_In_NoDup -?hd_error_skipn_iff_In;
+    [ eapply PCUICAst.NoDup_on_global_decls, H
+    | eexists; eassumption ]. }
+  { destruct p as [Σ ?]; cbn in *.
+    match goal with H : PCUICSN.NormalisationIn _ |- _ => revert H end.
+    move => normalisation_in.
+    rewrite referenced_impl_env_iter_pop_eq.
+    repeat match goal with H : _ |- _ => rewrite referenced_impl_env_iter_pop_eq in H end.
+    eapply normalisation_in_adjust_universes in normalisation_in; eauto; revgoals.
+    { repeat match goal with H : PCUICTyping.wf_ext _ |- _ => destruct H end;
+        split; eassumption. }
+    { let H := multimatch goal with H : PCUICTyping.wf_ext _ |- _ => H end in
+      rewrite /PCUICAst.PCUICEnvironment.lookup_env -PCUICAst.PCUICEnvironment.lookup_global_Some_iff_In_NoDup -?hd_error_skipn_iff_In;
+      [ eapply PCUICAst.NoDup_on_global_decls, H
+      | eexists; eassumption ]. }
+    revert normalisation_in.
+    apply PCUICWeakeningEnvSN.weakening_env_normalisation_in; eauto;
+      try match goal with H : PCUICTyping.wf_ext _ |- _ => refine (@PCUICTyping.wf_ext_wf _ _ H) end.
+    apply PCUICAst.PCUICEnvironment.extends_decls_extends; split; cbn; try reflexivity.
+    eauto using firstn_skipn. }
+Qed.
+
+Program Definition erase_pcuic_program {guard : abstract_guard_impl} (p : pcuic_program)
+  {normalisation_in : NormalisationIn_erase_pcuic_program_1 p}
+  {normalisation_in_adjust_universes : NormalisationIn_erase_pcuic_program_2 p}
   (wfΣ : ∥ PCUICTyping.wf_ext (H := config.extraction_checker_flags) p.1 ∥)
   (wt : ∥ ∑ T, PCUICTyping.typing (H := config.extraction_checker_flags) p.1 [] p.2 T ∥) : eprogram_env :=
   let wfe := build_wf_env_from_env p.1.1 (map_squash (PCUICTyping.wf_ext_wf _) wfΣ) in
   let wfext := @abstract_make_wf_env_ext _ optimized_abstract_env_impl wfe p.1.2 _ in
-  let t := ErasureFunction.erase (nor:=PCUICSN.extraction_normalizing) (normalisation_in:=let _ := @PCUICSN.normalisation in _) optimized_abstract_env_impl wfext nil p.2
+  let t := ErasureFunction.erase (normalisation_in:=_) optimized_abstract_env_impl wfext nil p.2
     (fun Σ wfΣ => let '(sq (T; ty)) := wt in PCUICTyping.iswelltyped ty) in
-  let Σ' := ErasureFunction.erase_global_fast (nor:=PCUICSN.extraction_normalizing) (normalisation:=normalisation) optimized_abstract_env_impl
+  let Σ' := ErasureFunction.erase_global_fast (normalisation_in:=_) optimized_abstract_env_impl
     (EAstUtils.term_global_deps t) wfe (p.1.(PCUICAst.PCUICEnvironment.declarations)) _ in
     (EEnvMap.GlobalContextMap.make Σ' _, t).
 
+Next Obligation. unshelve edestruct erase_pcuic_program_normalisation_helper; cbn in *; eauto. Qed.
 Next Obligation.
   eapply wf_glob_fresh.
   eapply ErasureFunction.erase_global_fast_wf_glob.
+  unshelve edestruct erase_pcuic_program_normalisation_helper; cbn in *; eauto.
 Qed.
 
 Obligation Tactic := idtac.
 
 Import Extract.
 
-Definition erase_program {guard : abstract_guard_impl} {normalisation : PCUICSN.Normalisation} (p : pcuic_program)
-  (wtp : ∥ wt_pcuic_program (cf:=config.extraction_checker_flags) p ∥) : eprogram_env :=
-  erase_pcuic_program (guard := guard) p (map_squash fst wtp) (map_squash snd wtp).
+Definition erase_program {guard : abstract_guard_impl} (p : pcuic_program)
+  {normalisation_in normalisation_in_adjust_universes}
+  (wtp : ∥ wt_pcuic_program (cf:=config.extraction_checker_flags) p ∥)
+  : eprogram_env :=
+  @erase_pcuic_program guard p normalisation_in normalisation_in_adjust_universes (map_squash fst wtp) (map_squash snd wtp).
 
-Lemma expanded_erase_program {guard : abstract_guard_impl} {normalisation : PCUICSN.Normalisation}
-  (cf := config.extraction_checker_flags) p (wtp : ∥ wt_pcuic_program p ∥) :
+Lemma expanded_erase_program {guard : abstract_guard_impl} p {normalisation_in normalisation_in_adjust_universes} (wtp : ∥ wt_pcuic_program p ∥) :
   PCUICEtaExpand.expanded_pcuic_program p ->
-  EEtaExpandedFix.expanded_eprogram_env (erase_program (guard:=guard) p wtp).
+  EEtaExpandedFix.expanded_eprogram_env (@erase_program guard p normalisation_in normalisation_in_adjust_universes wtp).
 Proof.
   intros [etaenv etat]. split;
-  unfold erase_program, erase_pcuic_program; cbn.
-  eapply ErasureFunction.expanded_erase_global_fast, etaenv; reflexivity.
+  unfold erase_program, erase_pcuic_program.
+  eapply ErasureFunction.expanded_erase_global_fast, etaenv; try reflexivity; eauto.
+  unshelve edestruct erase_pcuic_program_normalisation_helper; cbn in *; eauto.
   apply: (ErasureFunction.expanded_erase_fast (X_type:=optimized_abstract_env_impl)).
+  unshelve edestruct erase_pcuic_program_normalisation_helper; cbn in *; eauto.
   reflexivity. exact etat.
 Qed.
 
@@ -67,33 +189,50 @@ Proof.
   - eapply EEtaExpanded.isEtaExpFix_isEtaExp. now eapply EEtaExpandedFix.expanded_isEtaExp.
 Qed.
 
-Program Definition erase_transform {guard : abstract_guard_impl} {normalisation : PCUICSN.Normalisation} : Transform.t pcuic_program eprogram_env PCUICAst.term EAst.term
+Obligation Tactic := try solve [ eauto ].
+
+Program Definition erase_transform {guard : abstract_guard_impl} : Transform.t pcuic_program eprogram_env PCUICAst.term EAst.term
   eval_pcuic_program (eval_eprogram_env EWcbvEval.default_wcbv_flags) :=
  {| name := "erasure";
     pre p :=
-      ∥ wt_pcuic_program (cf := config.extraction_checker_flags) p ∥ /\ PCUICEtaExpand.expanded_pcuic_program p ;
-    transform p hp := erase_program (guard:=guard) p (proj1 hp) ;
+     ∥ wt_pcuic_program (cf := config.extraction_checker_flags) p ∥
+     /\ PCUICEtaExpand.expanded_pcuic_program p
+     /\ NormalisationIn_erase_pcuic_program_1 p
+     /\ NormalisationIn_erase_pcuic_program_2 p ;
+   transform p hp := let nhs := proj2 (proj2 hp) in
+                     @erase_program guard p (proj1 nhs) (proj2 nhs) (proj1 hp) ;
     post p := [/\ wf_eprogram_env all_env_flags p & EEtaExpandedFix.expanded_eprogram_env p];
-    obseq g g' v v' := let Σ := g.1 in Σ ;;; [] |- v ⇝ℇ v' |}.
+   obseq g g' v v' := let Σ := g.1 in Σ ;;; [] |- v ⇝ℇ v' |}.
+
 Next Obligation.
   cbn -[erase_program].
-  intros ? ? p [wtp etap].
+  intros ? p (wtp&etap&?&?).
   destruct erase_program eqn:e.
-  split; cbn.
-  - unfold erase_program, erase_pcuic_program in e. simpl. cbn in e. injection e. intros <- <-.
+  split.
+  - unfold erase_program, erase_pcuic_program in e.
+    set (egf := ErasureFunction.erase_global_fast _ _ _ _ _) in e.
+    set (ef := ErasureFunction.erase _ _ _ _ _) in e.
+    cbn -[egf ef] in e. injection e. intros <- <-.
     split.
-    eapply ErasureFunction.erase_global_fast_wf_glob.
-    apply: (ErasureFunction.erase_wellformed_fast (X_type:=optimized_abstract_env_impl)).
+    eapply ErasureFunction.erase_global_fast_wf_glob; eauto;
+      try match goal with H : _ |- _ => eapply H end.
+    unshelve edestruct erase_pcuic_program_normalisation_helper; cbn in *; eauto.
+    apply: (ErasureFunction.erase_wellformed_fast (X_type:=optimized_abstract_env_impl)); eauto;
+      try match goal with H : _ |- _ => eapply H end.
+    unshelve edestruct erase_pcuic_program_normalisation_helper; cbn in *; eauto.
   - rewrite -e. cbn.
     now eapply expanded_erase_program.
 Qed.
 
 Next Obligation.
-  red. move=> guard normalisation [Σ t] v [[wf [T HT]]]. unfold eval_pcuic_program, eval_eprogram.
+  red. move=> guard p v [[wf [T [HT1 HT2]]]]. unfold eval_pcuic_program, eval_eprogram.
+  unshelve edestruct erase_pcuic_program_normalisation_helper; cbn in *; try now destruct wf; eauto.
+  destruct p as [Σ t].
   intros [ev].
   destruct erase_program eqn:e.
   unfold erase_program, erase_pcuic_program in e. simpl in e. injection e; intros <- <-.
   simpl. clear e. cbn in *.
+  destruct wf; cbn in *.
   set (Σ' := build_wf_env_from_env _ _).
   assert (ev' :forall Σ0 : PCUICAst.PCUICEnvironment.global_env, Σ0 = Σ' -> PCUICWcbvEval.eval Σ0 t v).
   { intros; now subst. }
@@ -103,8 +242,19 @@ Next Obligation.
   2:eapply Kernames.KernameSet.subset_spec; reflexivity.
   destruct ev' as [v' [he [hev]]]. exists v'; split => //.
   red. cbn.
-  sq. exact hev. Unshelve. cbn; intros. now subst.
+  sq. exact hev. Unshelve.
+  { intros; cbn in *.
+    subst Σ'.
+    multimatch goal with
+    | [ H : _ |- _ ] => eapply H
+    end; try eassumption;
+    rewrite referenced_impl_env_iter_pop_eq;
+    repeat match goal with H : _ |- _ => rewrite referenced_impl_env_iter_pop_eq in H end;
+    assumption. }
+  cbn; intros. sq. now subst.
 Qed.
+
+Obligation Tactic := idtac.
 
 (** This transformation is the identity on terms but changes the evaluation relation to one
     where fixpoints are not guarded. It requires eta-expanded fixpoints and evaluation
